generalize two state reasoning to a list of steps

TwoState.dfy
@@ -1,10 +1,12 @@
 include "../armada/code/dafny/fl/spec/refinement.s.dfy"
 include "../armada/code/dafny/fl/util/refinement/AnnotatedBehavior.i.dfy"
+include "../armada/code/dafny/util/collections/seqs.i.dfy"
 
 module TwoStateModule {
     import opened GeneralRefinementModule
     import opened AnnotatedBehaviorModule
     import opened util_collections_seqs_s
+    import opened util_collections_seqs_i
 
     datatype ActorTriple<S, T> = ActorTriple(s: S, s': S, actor: T)
 
@@ -69,26 +71,32 @@ module TwoStateModule {
             ==> (StateActorPair(s, tid) in pc1 <==> StateActorPair(s', tid) in pc2)
     }
     
+    predicate AllActionsHaveActor<A,T>(idmap: imap<A, T>, trace: seq<A>, tid: T)
+    {
+        forall i :: 0 <= i < |trace| ==> trace[i] in idmap && idmap[trace[i]] == tid
+    }
+
     predicate HoareLogicAssumptions<S,A,T>(r: YieldRequest<S, A, T>, their_states: seq<S>, my_states: seq<S>, trace: seq<A>)
     {
-        && |their_states| - 1 == |my_states| == |trace|
+        && |their_states| == |my_states| == |r.pcs| == |trace| + 1
         && |trace| > 0
         && trace[0] in r.idmap 
         && var tid := r.idmap[trace[0]];
-        && (forall i :: 0 <= i < |trace| ==> trace[i] in r.idmap && r.idmap[trace[0]] == tid)
-        && StateActorPair(s0, tid) in r.pre
-        && ActorTriple(s0, s1, tid) in r.Y
-        && StateActorPair(s1, tid) in r.pcs[i]
-        && ActionTriple(s1, s2, a) in r.next
-        && ActorTriple(s2, s3, tid) in r.Y
-
+        && AllActionsHaveActor(r.idmap, trace, tid)
+        && StateActorPair(their_states[0], tid) in r.pre
+        && (forall i :: 0 <= i < |their_states| ==>
+            ActorTriple(their_states[i], my_states[i], tid) in r.Y)
+        && (forall i :: 0 <= i < |their_states| - 1 ==>
+            ActionTriple(my_states[i], their_states[i+1], trace[i]) in r.next)
+        && (forall i :: 0 <= i < |my_states| ==>
+            StateActorPair(my_states[i], tid) in r.pcs[i])
     }
 
     predicate HoareLogic<S,A,T>(r: YieldRequest<S, A, T>)
     {
-        forall s0, s1, s2, s3, a ::
-            HoareLogicAssumptions(r, s0, s1, s2, s3, a, i)
-            ==> StateActorPair(s3, r.idmap[a]) in r.post
+        forall their_states, my_states, trace ::
+            HoareLogicAssumptions(r, their_states, my_states, trace)
+            ==> StateActorPair(last(my_states), r.idmap[trace[0]]) in r.post
     }
 
     predicate ValidYieldRequest<S,A,T>(r: YieldRequest<S, A, T>)
@@ -106,32 +114,42 @@ module TwoStateModule {
         && (forall a' :: a' in trace && a' in idmap ==> idmap[a'] != tid)
     }
 
-    predicate BehaviorLogicAssumptions<S, A, T>(r: YieldRequest<S, A, T>, states0: seq<S>, trace0: seq<A>, states1: seq<S>, trace1: seq<A>, a: A)
+    predicate BehaviorLogicAssumptions<S, A, T>(r: YieldRequest<S, A, T>, states: seq<(seq<S>, seq<A>)>, trace: seq<A>)
     {
-        && a in r.idmap 
-        && var tid := r.idmap[a]; 
-        && RelyStateNextSeq(r.next, r.idmap, states0, trace0, tid)
-        && RelyStateNextSeq(r.next, r.idmap, states1, trace1, tid)
-        && StateActorPair(states0[0], tid) in r.pre
-        && StateActorPair(last(states0), tid) in r.pc
-        && ActionTriple(last(states0), states1[0], a) in r.next
+        && |states| == |r.pcs| == |trace| + 1
+        && |trace| > 0
+        && trace[0] in r.idmap
+        && var tid := r.idmap[trace[0]];
+        && AllActionsHaveActor(r.idmap, trace, tid)
+        && (forall i :: 0 <= i < |states| ==>
+            var (s,t) := states[i];
+            && RelyStateNextSeq(r.next, r.idmap, s, t, tid)
+            && StateActorPair(last(s), tid) in r.pcs[i])
+        && StateActorPair(states[0].0[0], tid) in r.pre
+        && (forall i :: 0 <= i < |trace| ==>
+            ActionTriple(last(states[i].0), states[i+1].0[0], trace[i]) in r.next)
     }
 
     predicate BehaviorLogic<S, A, T>(r: YieldRequest<S, A, T>)
     {
-        forall states0, trace0, states1, trace1, a :: 
-            BehaviorLogicAssumptions(r, states0, trace0, states1, trace1, a)
-            ==> StateActorPair(last(states1), r.idmap[a]) in r.post
+        forall states, trace ::
+            BehaviorLogicAssumptions(r, states, trace)
+            ==> StateActorPair(last(last(states).0), r.idmap[trace[0]]) in r.post
     }
 
-    lemma lemma_UseHoareLogic<S,A,T>(r: YieldRequest<S, A, T>, s0: S, s1: S, s2: S, s3: S, a: A)
+    lemma lemma_UseHoareLogic<S,A,T>(
+        r: YieldRequest<S, A, T>,
+        their_states: seq<S>,
+        my_states: seq<S>,
+        trace: seq<A>
+        )
         requires HoareLogic(r)
-        requires HoareLogicAssumptions(r, s0, s1, s2, s3, a)
-        ensures StateActorPair(s3, r.idmap[a]) in r.post
+        requires HoareLogicAssumptions(r, their_states, my_states, trace)
+        ensures StateActorPair(last(my_states), r.idmap[trace[0]]) in r.post
     {}
 
     lemma lemma_YieldAbstractsNextSequence<S,A,T>(
-        next: iset<ActionTriple<S,A>>, 
+        next: iset<ActionTriple<S,A>>,
         Y: iset<ActorTriple<S,T>>, 
         idmap: imap<A, T>, 
         states: seq<S>, 
@@ -158,24 +176,25 @@ module TwoStateModule {
 
     lemma lemma_UseYieldPredicate<S,A,T>(
         r: YieldRequest<S, A, T>, 
-        states0: seq<S>, 
-        trace0: seq<A>, 
-        states1: seq<S>, 
-        trace1: seq<A>, 
-        a: A
+        states: seq<(seq<S>, seq<A>)>,
+        trace: seq<A>
         )
         requires ValidYieldRequest(r)
-        requires BehaviorLogicAssumptions(r, states0, trace0, states1, trace1, a)
-        ensures StateActorPair(last(states1), r.idmap[a]) in r.post
+        requires BehaviorLogicAssumptions(r, states, trace)
+        ensures StateActorPair(last(last(states).0), r.idmap[trace[0]]) in r.post
     {
-        var tid := r.idmap[a];
-        var s0 := states0[0];
-        var s1 := last(states0);
-        var s2 := states1[0];
-        var s3 := last(states1);
+        var tid := r.idmap[trace[0]];
 
-        lemma_YieldAbstractsNextSequence(r.next, r.Y, r.idmap, states0, trace0, tid);
-        lemma_YieldAbstractsNextSequence(r.next, r.Y, r.idmap, states1, trace1, tid);
-        lemma_UseHoareLogic(r, s0, s1, s2, s3, a);
+        forall i | 0 <= i < |states|
+            ensures ActorTriple(states[i].0[0], last(states[i].0), tid) in r.Y
+        {
+            var (s, t) := states[i];
+            lemma_YieldAbstractsNextSequence(r.next, r.Y, r.idmap, s, t, tid);
+        }
+
+        var their_states := ConvertMapToSeq(|states|, map i | 0 <= i < |states| :: states[i].0[0]);
+        var my_states := ConvertMapToSeq(|states|, map i | 0 <= i < |states| :: last(states[i].0));
+
+        lemma_UseHoareLogic(r, their_states, my_states, trace);
     }
 }
